\documentclass{article}
% \usepackage{graphicx}
\usepackage{amsthm}
\usepackage{amsmath}

\title{HW4 (CSCI-C241)}
\author{Lillie Donato}
\date{6 February 2024}

\usepackage{geometry}
\geometry{a4paper, total={170mm,257mm}, left=20mm, top=20mm}

\begin{document}

\maketitle

\begin{enumerate}
    \item Question One
    \begin{enumerate}
        \item This proof is valid.
        \item This proof is not valid, as in their proof by contradiction, they are not proving the entire conclusion and only one part of it.
        \item This proof is valid.
        \item This proof is valid.
    \end{enumerate}
    \item Question Two
    \begin{enumerate}
        \item
        Claim: $P \land Q \vdash \neg (P \rightarrow \neg Q)$ \\
        Goal: $\neg (P \rightarrow \neg Q)$
        \begin{proof}[Pf: Assume $P \land Q$]
            \begin{align*}
                &1. \quad \text{From } P \land Q, \text{ we can conclude } P \text{ and } Q && \text{($\land - Elimination$)} \\
                &2. \quad Subproof \\
                &3. \quad \hspace{1cm} \text{Suppose towards a contradiction that } P \rightarrow \neg Q \\
                &4. \quad \hspace{1cm} \text{From } P, \text{ we can apply } P \rightarrow \neg Q \text{ and conclude } \neg Q && \text{(Application)} \\
                &5. \quad \text{Under the assumption of } P \rightarrow \neg Q, \text{ we proved an impossibility, } \\
                &\quad \text{so therefore } \neg(P \rightarrow \neg Q) && \text{(Proof By Contradiction)}
            \end{align*}
        \end{proof}
        \item
        Claim: $\vdash \neg ((P \land Q) \land (P \rightarrow \neg Q))$ \\
        Goal: $\neg (X \land Z)$
        \begin{proof}[Proof]
            \begin{align*}
                &1. \quad Subproof \\
                &2. \quad \hspace{1cm} \text{Suppose } (P \land Q) \land (P \rightarrow \neg Q) \text{ towards a contradiction} \\
                &3. \quad \hspace{1cm} \text{From } (P \land Q) \land (P \rightarrow \neg Q), \text{ we can conclude } P \land Q \text{ and } P \rightarrow \neg Q && \text{($\land - Elimination$)} \\
                &4. \quad \hspace{1cm} \text{From } P \land Q, \text{ we can conclude } P \text{ and } Q && \text{($\land - Elimination$)} \\
                &5. \quad \hspace{1cm} \text{From } P, \text{ we can apply } P \rightarrow \neg Q \text{ and conclude } \neg Q && \text{(Application)} \\
                &6. \quad \text{Under the assumption of } (P \land Q) \land (P \rightarrow \neg Q) \text{ we proved an impossibility of } \\
                &\quad Q \text{ and } \neg Q \text{ so therefore } \neg ((P \land Q) \land (P \rightarrow \neg Q)) && \text{(Proof By Contradiction)} \\
            \end{align*}
        \end{proof}
        \item With the truth assignment ($A = false$, $B = true$), the proof is invalid.
        \item
        Claim: $(W \land X) \rightarrow \neg Y, X \vdash \neg (W \land Y)$ \\
        Goal: $\neg (W \land Y)$
        \begin{proof}[Assume $(W \land X) \rightarrow \neg Y, X$]
            \begin{align*}
                &1. \quad Subproof \\
                &2. \quad \hspace{1cm} \text{Suppose } W \land Y \text{ towards a contradiction} \\
                &3. \quad \hspace{1cm} \text{From } W \land Y, \text{ we can conclude } W \text{ and } Y && \text{($\land - Elimination$)} \\
                &4. \quad \hspace{1cm} \text{From } W \text{ and } X, \text{ we can conclude } W \land X && \text{($\land - Introduction$)} \\
                &5. \quad \hspace{1cm} \text{From } W \land X, \text{ we can apply } (W \land X) \rightarrow \neg Y \text{ and conclude } \neg Y && \text{(Application)} \\
                &6. \quad \text{Under the assumption of } W \land Y \text{ we proved an impossibility of } Y \text{ and } \neg Y \\
                &\quad \text{ so therefore } \neg (W \land Y) && \text{(Proof By Contradiction)} \\
            \end{align*}
        \end{proof}
        \item
        Claim: $(W \land X) \rightarrow \neg Y \vdash X \rightarrow \neg (W \land Y)$ \\
        Goal: $X \rightarrow \neg (W \land Y)$
        \begin{proof}[Assume $(W \land X) \rightarrow \neg Y$]
            \begin{align*}
                &1. \quad \text{Assume } X \\
                &2. \quad \hspace{1cm} \text{Suppose } W \land Y \text{ towards a contradiction} \\
                &3. \quad \hspace{2cm} \text{From } W \land Y, \text{ we can conclude } W \text{ and } Y && \text{($\land - Elimination$)} \\
                &4. \quad \hspace{2cm} \text{From } W \text{ and } X, \text{ we can conclude } W \land X && \text{($\land - Introduction$)} \\
                &5. \quad \hspace{2cm} \text{From } W \land X, \text{ we can apply } (W \land X) \rightarrow \neg Y \text{ and conclude } \neg Y && \text{(Application)} \\
                &6. \quad \hspace{1cm} \text{Under the assumption of } W \land Y \text{ we proved an impossibility of } Y \text{ and } \neg Y \\
                &\quad \text{ so therefore } \neg (W \land Y) && \text{(Proof By Contradiction)} \\
                &7. \quad \text{Under the assumption of } X, \text{ we proved } \neg (W \land Y), \text{ so therefore } X \rightarrow \neg (W \land Y) && \text{(Direct Proof)}
            \end{align*}
        \end{proof}
        \item
        Claim: $U \rightarrow V, \neg V \vdash \neg (U \land W)$ \\
        Goal: $\neg (U \land W)$
        \begin{proof}[Assume $U \rightarrow V, \neg V$]
            \begin{align*}
                &1. \quad Subproof \\
                &2. \quad \hspace{1cm} \text{Suppose } U \land W \text{ towards a contradiction} \\
                &3. \quad \hspace{1cm} \text{From } U \land W, \text{ we can conclude } U \text{ and } W && \text{($\land - Elimination$)} \\
                &4. \quad \hspace{1cm} \text{From } U, \text{ we can apply } U \rightarrow V \text{ and conclude } V && \text{(Application)} \\
                &5. \quad \text{Under the assumption of } U \land W \text{ we proved an impossibility of } V \text{ and } \neg V \\
                &\quad \text{ so therefore } \neg (U \land W) && \text{(Proof By Contradiction)}
            \end{align*}
        \end{proof}
        \item With the truth assignment ($U = false$, $V = false, W = true$), the proof is invalid.
        \item
        Claim: $U \rightarrow V, W \rightarrow V, \neg V \vdash \neg U \land \neg W$ \\
        Goal: $\neg U \land \neg W$
        \begin{proof}[Assume $U \rightarrow V, W \rightarrow V, \neg V$]
            \begin{align*}
                &1. \quad Subproof \\
                &2. \quad \hspace{1cm} \text{Suppose } U \text{ towards a contradiction} \\
                &3. \quad \hspace{1cm} \text{From } U, \text{ we can apply } U \rightarrow V \text{ and conclude } V && \text{(Application)} \\
                &4. \quad \text{Under the assumption of } U \text{ we proved an impossibility of } V \text{ and } \neg V \\
                &\quad \text{ so therefore } \neg U && \text{(Proof By Contradiction)} \\
                &5. \quad Subproof \\
                &6. \quad \hspace{1cm} \text{Suppose } W \text{ towards a contradiction} \\
                &7. \quad \hspace{1cm} \text{From } W, \text{ we can apply } W \rightarrow V \text{ and conclude } V && \text{(Application)} \\
                &8. \quad \text{Under the assumption of } U \text{ we proved an impossibility of } V \text{ and } \neg V \\
                &\quad \text{ so therefore } \neg W && \text{(Proof By Contradiction)} \\
                &9. \quad \text{From } \neg U \text{ and } \neg W, \text{ we can conclude } \neg U \land \neg W && \text{($\land - Introduction$)}
            \end{align*}
        \end{proof}
    \end{enumerate}
    \item Question Three
    \begin{enumerate}
        \item This would be true because the main connective in this statement holds the same meaning as the word "and".
        \item This would not be the case, as there are no assignments that satisfy both $A$ and $\neg A$, but there are assignments that satisfy $B \leftrightarrow (X \oplus \neg Q)$.
        \item This argument would be valid for the reason that there are no assignments where the premises are satisfied and the conclusion is not.
        \item Yes, it would be possible but only if the premises were contradictions as well.
        \item Yes, this would be possible but only if that other formula was also a contradiction.
    \end{enumerate}
    \item Question Four \\
    Claim: $\vdash P \lor \neg P$ \\
    Goal: $P \lor \neg P$
    \begin{proof}
        \begin{align*}
            &1. \quad \text{Suppose } \neg (P \lor \neg P) \text{ towards a contradiction} \\
            &2. \quad \hspace{1cm} \text{Suppose } P \text{ towards a contradiction} \\
            &3. \quad \hspace{2cm} \text{From } P, \text{ we can conclude } P \lor \neg P && \text{(Weakening)} \\
            &4. \quad \hspace{1cm} \text{Under the assumption of } P \text{ we proved an impossibility of } \\
            &(P \lor \neg P) \land \neg (P \lor \neg P) \text{ so therefore } \neg P && \text{(Proof By Contradiction)} \\
            &5. \quad \hspace{1cm} \text{From } P, \text{ we can conclude } P \lor \neg P && \text{(Weakening)} \\
            &6. \quad \text{Under the assumption of } \neg (P \lor \neg P) \text{ we proved and impossibility of } \\
            &(P \lor \neg P) \land \neg (P \lor \neg P), \text{ so therefore } P \lor \neg P && \text{(Proof By Contradiction)}
        \end{align*}
    \end{proof}
    \item Question Five
    \begin{enumerate}
        \item
        Claim: $(A \rightarrow B) \rightarrow C \equiv (\neg A \rightarrow C) \land (B \rightarrow C)$
        \begin{proof}[Pf: Assume $(A \rightarrow B) \rightarrow C \equiv (\neg A \rightarrow C) \land (B \rightarrow C)$]
            \begin{align*}
                &1. \quad (A \rightarrow B) \rightarrow C && \equiv \neg (\neg A \lor B) \lor C && \text{(Material Implication)}\\
                &2. \quad && \equiv (\neg \neg A \land \neg B) \lor C && \text{(De Morgan's)} \\
                &3. \quad && \equiv (A \land \neg B) \lor C && \text{(Double Negation)} \\
                &4. \quad (\neg A \rightarrow C) \land (B \rightarrow C) && \equiv (\neg \neg A \lor C) \land (\neg B \lor C) && \text{(Material Implication)} \\
                &5. \quad && \equiv (A \lor C) \land (\neg B \lor C) && \text{(Double Negation)} \\
                &6. \quad && \equiv (A \land \neg B) \lor C && \text{(Distributive)}
            \end{align*}
        \end{proof}
        \item With the truth assignment ($A = true$, $B = false$, $C = false$), the two formulas are not equivlaent.
        \item With the truth assignment ($W = true$, $X = false$, $Y = true$, $Z = false$), the two formulas are not equivlaent.
        \item
        Claim: $\neg ((W \land \neg X) \rightarrow (\neg Y \lor Z)) \equiv (Y \land \neg Z) \land (W \land \neg X)$
        \begin{proof}[Pf: Assume $\neg ((W \land \neg X) \rightarrow (\neg Y \lor Z)) \equiv (Y \land \neg Z) \land (W \land \neg X)$]
            \begin{align*}
                &1. \quad \neg ((W \land \neg X) \rightarrow (\neg Y \lor Z)) && \equiv \neg (\neg (W \land \neg X) \lor (\neg Y \lor Z)) && \text{(Material Implication)} \\
                &2. \quad && \equiv \neg ((\neg W \lor \neg \neg X) \lor (\neg Y \lor Z)) && \text{(De Morgan's)} \\
                &3. \quad && \equiv (\neg (\neg W \lor \neg \neg X) \land \neg (\neg Y \lor Z)) && \text{(De Morgan's)} \\
                &4. \quad && \equiv (\neg (\neg W \lor X) \land \neg (\neg Y \lor Z)) && \text{(Double Negation)} \\
                &5. \quad && \equiv (\neg \neg W \land \neg X) \land (\neg \neg Y \land \neg Z) && \text{(De Morgan's)} \\
                &6. \quad && \equiv (W \land \neg X) \land (Y \land \neg Z) && \text{(Double Negation)} \\
                &7. \quad && \equiv (Y \land \neg Z) \land (W \land \neg X) && \text{(Commutative)}
            \end{align*}
        \end{proof}
        \item
        Claim: $P \land (\neg Q \rightarrow R) \equiv (P \rightarrow \neg R) \rightarrow (P \land Q)$
        \begin{proof}[Pf: Assume $P \land (\neg Q \rightarrow R) \equiv (P \rightarrow \neg R) \rightarrow (P \land Q)$]
            \begin{align*}
                &1. \quad P \land (\neg Q \rightarrow R) && \equiv P \land (\neg \neg Q \lor R) && \text{(Material Implication)} \\
                &2. \quad && \equiv P \land (Q \lor R) && \text{(Double Negation)} \\
                &3. \quad (P \rightarrow \neg R) \rightarrow (P \land Q) && \equiv \neg (\neg P \lor \neg R) \lor (P \land Q) && \text{(Material Implication)} \\
                &4. \quad && \equiv (\neg \neg P \land \neg \neg R) \lor (P \land Q) && \text{(De Morgan's)} \\
                &5. \quad && \equiv (P \land R) \lor (P \land Q) && \text{(Double Negation)} \\
                &6. \quad && \equiv P \land (Q \lor R) && \text{(Distributive)}
            \end{align*}
        \end{proof}
        \item
        Claim: $(M \rightarrow N) \land (\neg M \rightarrow N) \equiv N$
        \begin{proof}[Pf: Assume $(M \rightarrow N) \land (\neg M \rightarrow N) \equiv N$]
            \begin{align*}
                &1. \quad (M \rightarrow N) \land (\neg M \rightarrow N) && \equiv (\neg M \lor N) \land (\neg \neg M \lor N) && \text{(Material Implication)} \\
                &2. \quad && \equiv N \lor (\neg M \land \neg \neg M) && \text{(Distributive)} \\
                &3. \quad && \equiv N \lor (\neg M \land M) && \text{(Double Negation)} \\
                &4. \quad && \equiv N \lor \bot && \text{(Contradiction)} \\
                &5. \quad && \equiv N && \text{($\lor - Identity$)} \\
            \end{align*}
        \end{proof}
    \end{enumerate}
\end{enumerate}

\end{document}