\documentclass{article}
% \usepackage{graphicx}
\usepackage{amsthm}
\usepackage{amsmath}

\title{HW3 (CSCI-C241)}
\author{Lillie Donato}
\date{30 January 2024}

\usepackage{geometry}
\geometry{a4paper, total={170mm,257mm}, left=20mm, top=20mm}

\begin{document}

\maketitle

\begin{enumerate}
    \item Question One
    \begin{enumerate}
        \item This proof is not valid, for the reason that in line six, they are not acknowledging what was assumed in the subproof.
        \item This proof is valid.
        \item This proof is not valid, because after they do cases they wrote their direct proof incorrectly.
        \item This proof is valid.
        \item This proof is valid
        \item This proof is not valid, for that reason that when using $\lor - Elimination$, you must have a subproof for each case.
    \end{enumerate}

    \item Question Two
    \begin{enumerate}
        \item
        Claim: $(P \land Q) \rightarrow R, P \land S, \neg \neg Q \vdash R$ \\
        Goal: $R$ \\
        Want: $P \land Q$ \text{(Application)}
    
        \begin{proof}[Pf: Assume $(P \land Q) \rightarrow R, P \land S, \neg \neg Q$]
            \begin{align*}
                % &1. \quad \text{Assume } \neg \neg Q \\
                % &2. \quad \text{Therefore } && \text{Meow } \\
                &1. \quad \text{Since we know } \neg \neg Q, \text{ we can conclude } Q. && \text{(Double Negative)} \\
                &2. \quad \text{Since we know } P \land S, \text{ we can conclude } P. && \text{($\land - Elimination$)} \\
                &3. \quad \text{From } P \text{ and } Q, \text{ we can conclude } P \land Q. && \text{($\land - Introduction$)} \\
                &4. \quad \text{From } (P \land Q) \rightarrow R, P \text{ and } Q, \text{ we can conclude } R. && \text{($\rightarrow - Elimination$)} \\
                % Under the assumption of 
            \end{align*}
        \end{proof}

        \item
        Claim: $P \rightarrow \neg Q, \neg Q \vdash \neg \neg P$ \\
        Goal: $\neg \neg P$ \\
        \begin{tabular}{| c | c | c | c | c |}
            \hline
            $P$ & $Q$ & $P \rightarrow \neg Q$ & $\neg Q$ & $\neg \neg P$ \\
            \hline
            T & T & F & F & n/a \\
            \hline
            T & F & T & T & T \\
            \hline
            F & T & T & F & n/a \\
            \hline
            F & F & T & T & F \\
            \hline
        \end{tabular} \\

        This is not a valid argument, as shown in the following truth assignment:
        
        $P$ = $false$ \\
        $Q$ = $false$ \\
        $P \rightarrow \neg Q$ = $true$ \\
        $\neg Q$ = $true$ \\
        $\neg \neg P$ = $false$ \\

        \item
        Claim: $(A \land B) \rightarrow C, B, A \land \neg D \vdash C \land \neg D$ \\
        Goal: $C \land \neg D$
        \begin{proof}[Pf: Assume $(A \land B) \rightarrow C, B, A \land \neg D$]
            \begin{align*}
                &1. \quad \text{From } A \land \neg D, \text{ we can conclude } A \text{ and } \neg D. && \text{($\land - Elimination$)} \\
                &2. \quad \text{From } A \text{ and } B, \text{ we can conclude } A \land B. && \text{($\land - Introduction$)} \\
                &3. \quad \text{From } A \land B, \text{ we can apply } (A \land B) \rightarrow C \text{ and conclude } C. && \text{($Application$)} \\
                &4. \quad \text{From } A \text{ and } \neg D, \text{ we can conclude } A \land \neg D. && \text{($\land - Introduction$)} \\
            \end{align*}
        \end{proof}

        \item
        Claim: $(A \land B) \rightarrow C, B \vdash (A \land \neg D) \rightarrow (C \land \neg D)$ \\
        Goal: $(A \land \neg D) \rightarrow (C \land \neg D)$
        \begin{proof}[Pf: Assume $(A \land B) \rightarrow C, B$]
            \begin{align*}
                &1. \quad Subproof \\
                &2. \quad \hspace{1cm} \text{Assume } A \land \neg D. \\
                &3. \quad \hspace{1cm} \text{From } A \land \neg D, \text{ we can conclude } A \text{ and } \neg D. && \text{($\land - Elimination$)} \\
                &3. \quad \hspace{1cm} \text{From } A \text{ and } B, \text{ we can conclude } A \land B. && \text{($\land - Introduction$)} \\
                &4. \quad \hspace{1cm} \text{From } A \land B, \text{ we can apply } (A \land B) \rightarrow C \text{ and conclude } C. && \text{($Application$)} \\
                &5. \quad \hspace{1cm} \text{From } A \land \neg D \text{ we can apply } (A \land \neg D) \rightarrow (C \land \neg D) \text{ and conclude } C \land \neg D. && \text{($Application$)} \\
                &6. \quad \text{Under the assumption of } A \land \neg D, \text{ we proved } C \text{ and } \neg D. && \text{(Direct Proof)}
            \end{align*}
        \end{proof}

        \item
        Claim: $\neg P \rightarrow (Q \land R) \vdash (\neg P \land S) \rightarrow (R \land S)$ \\
        Goal: $(\neg P \land S) \rightarrow (R \land S)$
        \begin{proof}[Pf: Assume $\neg P \rightarrow (Q \land R)$]
            \begin{align*}
                &1. \quad Subproof \\
                &2. \quad \hspace{1cm} \text{Assume } \neg P \land S. \\
                &3. \quad \hspace{1cm} \text{From } \neg P \land S, \text{ we can conclude } \neg P \text{ and } S. && \text{($\land - Elimination$)} \\
                &4. \quad \hspace{1cm} \text{From } \neg P, \text{ we can apply } \neg P \rightarrow (Q \land R) \text{ and conclude } Q \land R. && \text{($Application$)} \\
                &5. \quad \hspace{1cm} \text{From } Q \land R, \text{ we can conclude } R. && \text{($\land - Elimination$)} \\
                &6. \quad \hspace{1cm} \text{From } \neg P \text{ and } S, \text{ we can conclude } \neg P \land S. && \text{($\land - Introduction$)} \\
                &7. \quad \hspace{1cm} \text{From } Q \land R \text{ we can conclude } Q \text{ and } R. && \text{($\land - Elimination$)} \\
                &8. \quad \hspace{1cm} \text{From } R \text{ and } S, \text{ we can conclude } R \land S. && \text{($\land - Introduction$)} \\
                &9. \quad \text{Under the assumption } \neg P \text{ and } S, \text{ we proved } R \land S, \text{ therefore } (\neg P \land S) \rightarrow (R \land S). && \text{(Direct Proof)} \\
            \end{align*}
        \end{proof}

        \item
        Claim: $X \land (X \rightarrow (Z \land Y)) \vdash X \land Y$ \\
        Goal: $X \land Y$
        \begin{proof}[Pf: Assume $X \land (X \rightarrow (Z \land Y))$]
            \begin{align*}
                &1. \quad \text{From } X \land (X \rightarrow (Z \land Y)) \text{ we can conclude } X \text{ and } X \rightarrow (Z \land Y) \\
                &2. \quad \text{From } X \text{ we can apply } X \rightarrow (Z \land Y) \text{ and conclude } Z \land Y. && \text{($Application$)} \\
                &3. \quad \text{From } Z \land Y \text{ we can conclude } Y. && \text{($\land - Elimination$)} \\
                &4. \quad \text{From } X \text{ and } Y \text{ we can conclude } X \land Y. && \text{($\land - Introduction$)} \\
            \end{align*}
        \end{proof}

        \item
        Claim: $\vdash (X \land (X \rightarrow (Z \land Y))) \rightarrow (X \land Y)$ \\
        Goal: $(X \land (X \rightarrow (Z \land Y))) \rightarrow (X \land Y)$
        \begin{proof}[Proof]
            \begin{align*}
                &1. \quad Subproof \\
                &2. \quad \hspace{1cm} \text{Assume } X \land (X \rightarrow (Z \land Y)) \\
                &3. \quad \hspace{1cm} \text{From } X \land (X \rightarrow (Z \land Y)) \text{ we can conclude } X \text{ and } X \rightarrow (Z \land Y) \\
                &4. \quad \hspace{1cm} \text{From } X \text{ we can apply } X \rightarrow (Z \land Y) \text{ and conclude } Z \land Y. && \text{($Application$)} \\
                &5. \quad \hspace{1cm} \text{From } Z \land Y \text{ we can conclude } Y. && \text{($\land - Elimination$)} \\
                &6. \quad \hspace{1cm} \text{From } X \text{ and } Y \text{ we can conclude } X \land Y. && \text{($\land - Introduction$)} \\
                &7. \quad \text{Under the assumption } X \land (X \rightarrow (Z \land Y)), \text{ we proved } (X \land Y), \\
                &\quad \text{ therefore } (X \land (X \rightarrow (Z \land Y))) \rightarrow (X \land Y) && \text{(Direct Proof)} \\
            \end{align*}
        \end{proof}

        \item
        Claim: $P \lor (Q \land \neg \neg R), P \rightarrow R \vdash R$ \\
        Goal: $R$
        \begin{proof}[Pf: Assume $P \lor (Q \land \neg \neg R), P \rightarrow R$]
            \begin{align*}
                &1. \quad \text{Case 1: } P \\
                &2. \quad \hspace{1cm} \text{From } P, \text{ we can apply } P \rightarrow R, \text{ and conclude } R. && \text{($Application$)} \\
                &3. \quad \text{Case 2: } Q \land \neg \neg R \\
                &4. \quad \hspace{1cm} \text{From } Q \land \neg \neg R, \text{ we can conclude } \neg \neg R. && \text{($\land - Elimination$)} \\
                &5. \quad \hspace{1cm} \text{From } \neg \neg R, \text{ we can conclude } R. && \text{(Double Negation)} \\
                &6. \quad \text{In either case of } P \lor (Q \land \neg \neg R), \text{ we proved } R, \text{ so } R \text{ is true in general.} && \text{(Proof By Cases)}
            \end{align*}
        \end{proof}

        \item
        Claim: $C \rightarrow (D \lor E), D \rightarrow E, \neg \neg C \vdash E \land C$ \\
        Goal: $E \land C$
        \begin{proof}[Pf: Assume $C \rightarrow (D \lor E), D \rightarrow E, \neg \neg C$]
            \begin{align*}
                &1. \quad \text{From } \neg \neg C, \text{ we can conclude } C. && \text{(Double Negation)} \\
                &2. \quad \text{From } C, \text{ we can apply } C \rightarrow (D \lor E), \text{ and conclude } D \lor E. && \text{($Application$)} \\
                &3. \quad \text{Case 1: } D \\
                &4. \quad \hspace{1cm} \text{From } D, \text{ we can apply } D \rightarrow E, \text{ and conclude } E. && \text{($Application$)} \\
                &5. \quad \text{Case 2: } E \\
                &6. \quad \hspace{1cm} \text{We know } E. \\
                &7. \quad \text{In either case of } D \lor E, \text{ we proved } E, \text{ so } E \text{ is true in general.} && \text{(Proof By Cases)} \\
                &8. \quad \text{From } E \text{ and } C, \text{ we can conclude } E \land C. && \text{($\land - Introduction$)}
            \end{align*}
        \end{proof}

        \item
        Claim: $X \rightarrow Y \vdash (X \lor Z) \rightarrow Y$ \\
        Goal: $(X \lor Z) \rightarrow Y$ \\
        \begin{tabular}{| c | c | c | c | c |}
            \hline
            $X$ & $Y$ & $Z$ & $X \rightarrow Y$ & $(X \lor Z) \rightarrow Y$ \\
            \hline
            $T$ & $T$ & $T$ & $T$ & true \\
            \hline
            $T$ & $T$ & $F$ & $T$ & true \\
            \hline
            $T$ & $F$ & $T$ & $F$ & n/a \\
            \hline
            $T$ & $F$ & $F$ & $F$ & n/a \\
            \hline
            $F$ & $T$ & $T$ & $T$ & true \\
            \hline
            $F$ & $T$ & $F$ & $T$ & true \\
            \hline
            $F$ & $F$ & $T$ & $T$ & false \\
            \hline
            $F$ & $F$ & $F$ & $T$ & true \\
            \hline
        \end{tabular}

        This is not a valid argument, as shown in the following truth assignment:
        
        $X$ = $false$ \\
        $Y$ = $false$ \\
        $Z$ = $true$ \\
        $X \rightarrow Y$ = $true$ \\
        $(X \lor Z) \rightarrow Y$ = $false$ \\

        \item
        Claim: $J \rightarrow K \vdash (J \lor \neg \neg K) \rightarrow K$ \\
        Goal: $(J \lor \neg \neg K) \rightarrow K$
        \begin{proof}[Pf: Assume $J \rightarrow K$]
            \begin{align*}
                &1. \quad Subproof \\
                &2. \quad \hspace{1cm} \text{Assume } J \lor \neg \neg K. \\
                &3. \quad \hspace{1cm} \text{Case 1: } J \\
                &4. \quad \hspace{2cm} \text{From } J, \text{ we can apply } J \rightarrow K, \text{ and conclude } K. && \text{($Application$)} \\
                &5. \quad \hspace{1cm} \text{Case 2: } \neg \neg K \\
                &6. \quad \hspace{2cm} \text{From } \neg \neg K, \text{ we can conclude } K. && \text{(Double Negation)} \\
                &7. \quad \hspace{1cm} \text{In either case of } J \lor \neg \neg K, \text{ we proved } K, \text{ so } K \text{ is true in general.} && \text{(Proof By Cases)} \\
                &8. \quad \text{Under the assumption } J \lor \neg \neg K, \text{ we proved } K, \text{ so therefore } (J \lor \neg \neg K) \rightarrow K. && \text{(Direct Proof)}\\
            \end{align*}
        \end{proof}
    \end{enumerate}
\end{enumerate}

\end{document}