\documentclass{article}
% \usepackage{graphicx}
\usepackage{amsthm}
\usepackage{amsmath}

\title{HW3 (Corrections) (CSCI-C241)}
\author{Lillie Donato}
\date{4 February 2024}

\usepackage{geometry}
\geometry{a4paper, total={170mm,257mm}, left=20mm, top=20mm}

\begin{document}

\maketitle

\begin{itemize}
    \item Question One
    \begin{itemize}
        \item 1c
        
        This proof is valid
        \item 1e
        
        This proof is not valid, as they are doing proof by cases, with cases that are part of an implication premise (meaning it's something that they do not have).
    \end{itemize}

    \item Question Two
    \begin{itemize}
        \item
        2d \\
        Claim: $(A \land B) \rightarrow C, B \vdash (A \land \neg D) \rightarrow (C \land \neg D)$ \\
        Goal: $(A \land \neg D) \rightarrow (C \land \neg D)$
        \begin{proof}[Pf: Assume $(A \land B) \rightarrow C, B$]
            \begin{align*}
                &1. \quad Subproof \\
                &2. \quad \hspace{1cm} \text{Assume } A \land \neg D. \\
                &3. \quad \hspace{1cm} \text{From } A \land \neg D, \text{ we can conclude } A \text{ and } \neg D. && \text{($\land - Elimination$)} \\
                &3. \quad \hspace{1cm} \text{From } A \text{ and } B, \text{ we can conclude } A \land B. && \text{($\land - Introduction$)} \\
                &4. \quad \hspace{1cm} \text{From } A \land B, \text{ we can apply } (A \land B) \rightarrow C \text{ and conclude } C. && \text{($Application$)} \\
                &5. \quad \hspace{1cm} \text{From } C \text{ and } \neg D, \text{ we can conclude } C \land \neg D. && \text{($\land - Introduction$)} \\
                &6. \quad \text{Under the assumption of } A \land \neg D, \text{ we proved } C \text{ and } \neg D. && \text{(Direct Proof)}
            \end{align*}
        \end{proof}
        
        \item
        2g \\
        Claim: $\vdash (X \land (X \rightarrow (Z \land Y))) \rightarrow (X \land Y)$ \\
        Goal: $(X \land (X \rightarrow (Z \land Y))) \rightarrow (X \land Y)$
        \begin{proof}[Proof]
            \begin{align*}
                &1. \quad Subproof \\
                &2. \quad \hspace{1cm} \text{Assume } X \land (X \rightarrow (Z \land Y))\\
                &3. \quad \hspace{1cm} \text{From } X \land (X \rightarrow (Z \land Y)) \text{ we can conclude } X \text{ and } X \rightarrow (Z \land Y) && \text{($\land - Elimination$)}  \\
                &4. \quad \hspace{1cm} \text{From } X \text{ we can apply } X \rightarrow (Z \land Y) \text{ and conclude } Z \land Y. && \text{($Application$)} \\
                &5. \quad \hspace{1cm} \text{From } Z \land Y \text{ we can conclude } Y. && \text{($\land - Elimination$)} \\
                &6. \quad \hspace{1cm} \text{From } X \text{ and } Y \text{ we can conclude } X \land Y. && \text{($\land - Introduction$)} \\
                &7. \quad \text{Under the assumption } X \land (X \rightarrow (Z \land Y)), \text{ we proved } (X \land Y), \\
                &\quad \text{ therefore } (X \land (X \rightarrow (Z \land Y))) \rightarrow (X \land Y) && \text{(Direct Proof)} \\
            \end{align*}
        \end{proof}
    \end{itemize}
\end{itemize}

\end{document}